\documentclass[pdftex,12pt,a4paper]{article}

\usepackage{wrapfig, amssymb, amsmath, graphicx, subfigure, pifont, seqsplit, float, booktabs, siunitx, adjustbox}
\usepackage[english]{babel}
\usepackage[top=1in, bottom=1in, left=1in, right=1in]{geometry}
\pagenumbering{arabic}
\newcommand{\HRule}{\rule{\linewidth}{0.5mm}}

\usepackage{forest}
\tikzset{el style/.style={midway, font=\scriptsize, inner sep=+1pt, auto=right}}
\forestset{angled/.style={
    content/.expanded={\noexpand\textless\forestov{content}\noexpand\textgreater}}}

\begin{document}
\input{title.tex}

\begin{enumerate}
    \item
        \begin{enumerate}
            \item $H(f(Y)) ? H(Y)$\\
                \begin{align}
                    H(Y) &= H(Y) + H[f(Y)|Y]\\
                         &= H(Y,f(Y))\\
                         &= H(f(Y)) + H(Y|f(Y))\\
                         &\ge H(f(Y))\\
                 H(f(Y)) &\le H(Y)
                \end{align}
            \item $H(X|f(Y)) ? H(X|Y)$
                \begin{align}
                    H(X|f(Y)) &? H(X|Y)\\
                    H(X,f(Y)) - H(f(Y)) &? H(X,Y) - H(Y)\\
                    H(f(Y)|X) + H(X) - H(f(Y)) &? H(Y|X) + H(X) - H(Y)\\
                    H(f(Y)|X) - H(f(Y)) &? H(Y|X) - H(Y)\\
                              &? H(Y,f(Y))\\
                              &? H(f(Y)) + H(Y|f(Y))\\
                              &\ge H(f(Y))\\
                 H(X|f(Y)) &\le H(X|Y)
                \end{align}
                NEEEDS WORK
            \item $I(X,Z|Y) = 0 \implies I(X;Z) ? I(X;Y)\mathrm{ \& }I(X;Z) ? I(Y;Z)$
                \begin{align}
                    I(X;Z|Y) &= I(X;Y,Z) - I(X;Y) = 0\\
                             &= I(X;Y|Z) + I(X;Z) - I(X;Y) = 0\\
                             &= I(X;Y|Z) + I(X;Z) = I(X;Y) \implies I(X;Z) \le I(X;Y)
                \end{align}
                \begin{align}
                    I(X;Z|Y) &= I(X;Y,Z) - I(X;Y) = 0\\
                             &= I(X;Y|Z) + I(X;Z) - I(X;Y) = 0\\
                             &= I(X;Z) = I(X;Y) - I(X;Y|Z)\\
                             \intertext{Chain rule for mutual information}
                             &= I(X;Z) = I(X;Y) - (I(X;Y) + H(Z|X) + H(Z|Y) - H(Z|X,Y) - H(Z))\\
                             &= I(X;Z) = - H(Z|X) - H(Z|Y) + H(Z|X,Y) + H(Z)\\
                             \intertext{$I(X;Y)= H(X,Y) - H(X|Y) - H(Y|X)$}
                             &= I(X;Z) + H(Z,Y) - H(Y|Z) = I(Z;Y) - H(Z|X) + H(Z|X,Y) + H(Z)\\
                             &= I(X;Z) + H(Z,Y) - H(Y|Z) + H(Z|X) - H(Z|X,Y) + H(Z) = I(Z;Y)\\
                             &= I(X;Z) + H(Z,Y) - (H(Y|Z) - H(Z)) + H(Z|X) - H(Z|X,Y) = I(Z;Y)\\
                             &= I(X;Z) + H(Z,Y) - H(Z,Y) + H(Z|X) - H(Z|X,Y) = I(Z;Y)\\
                             &= I(X;Z) + H(Z|X) - H(Z|X,Y) = I(Z;Y)\\
                             &= I(X;Z) - (-H(Z|X) + H(Z|X,Y)) = I(Z;Y)\\
                             &= I(X;Z) - (H(Z|X,Y) - H(Z|X)) = I(Z;Y)\\
                             &= I(X;Z) - H(Y|Z|X) = I(Z;Y)\\
                             &= I(X;Z) = I(Z;Y) + H(Y|Z|X)\\
                             &= I(X;Z) = I(Z;Y) + H(Y|Z|X) \implies I(X;Z) \ge I(Z;Y)
                \end{align}
                Too long but correct.
        \end{enumerate}
    \item 
    \item
\end{enumerate}

\end{document}
